src/ProgAuto.v
@@ -1,4 +1,4 @@
-Require Import BaseTypes Prog Simulation.
+Require Import BaseTypes Layer1 Simulation.
 Require Import Memx CommonAutomation.
 Require Import List.
 Require Import Eqdep.
@@ -9,54 +9,54 @@ Ltac invert_exec'' H :=
 
 Ltac invert_exec' :=
   match goal with
-  | [ H: exec _ (Ret _) _ _ |- _ ] =>
+  | [ H: exec _ (Ret _) _ |- _ ] =>
     invert_exec'' H
-  | [ H: exec _ (Read _) _ _ |- _ ] =>
+  | [ H: exec _ (Read _) _ |- _ ] =>
     invert_exec'' H
-  | [ H: exec _ (Write _ _) _ _ |- _ ] =>
-    invert_exec'' H
-  | [ H: exec _ (Seal _ _) _ _ |- _ ] =>
-    invert_exec'' H
-  | [ H: exec _ (Unseal _) _ _ |- _ ] =>
-    invert_exec'' H
-  | [ H: exec _ (Auth _) _ _ |- _ ] =>
+  | [ H: exec _ (Write _ _) _ |- _ ] =>
     invert_exec'' H
   end.
 
 Lemma bind_sep:
-  forall T T' st (p1: prog T) (p2: T -> prog T') ret tr',
-    exec st (Bind p1 p2) ret tr' ->
+  forall T T' st (p1: prog T) (p2: T -> prog T') ret,
+    exec st (Bind p1 p2) ret ->
     match ret with
     | Finished st' r =>
-    (exists tr1 tr2 r1 st1,
-       exec st p1 (Finished st1 r1) tr1 /\
-       exec st1 (p2 r1) ret tr2 /\ tr' = tr1 ++ tr2)
+    (exists r1 st1,
+       exec st p1 (Finished st1 r1) /\
+       exec st1 (p2 r1) ret)
   | Crashed st' =>
-    (exec st p1 (Crashed st') tr' \/
-     (exists tr1 tr2 r1 st1,
-        exec st p1 (Finished st1 r1) tr1 /\
-        exec st1 (p2 r1) ret tr2 /\ tr' = tr1 ++ tr2))
+    (exec st p1 (Crashed st') \/
+     (exists r1 st1,
+        exec st p1 (Finished st1 r1) /\
+        exec st1 (p2 r1) ret ))
+  | Failed st' =>
+    (exec st p1 (Failed st') \/
+     (exists r1 st1,
+        exec st p1 (Finished st1 r1) /\
+        exec st1 (p2 r1) ret ))
     end.
 Proof.
   intros.
   invert_exec'' H; eauto.
   destruct ret.
-  do 4 eexists; eauto.
-  right; do 4 eexists; eauto.
+  do 2 eexists; eauto.
+  right; do 2 eexists; eauto.
+  right; do 2 eexists; eauto.
 Qed.
 
 Ltac invert_exec :=
   match goal with
-  |[H : exec _ (Bind _ _) _ _ |- _ ] =>
+  |[H : exec _ (Bind _ _) _ |- _ ] =>
    apply bind_sep in H; repeat cleanup
-  |[H : exec _ _ _ _ |- _ ] =>
+  |[H : exec _ _ _ |- _ ] =>
    invert_exec'
   end.
 
 
   Definition prog_equiv T : prog T -> prog T -> Prop :=
-    fun p1 p2 => forall st tr' out,
-        exec st p1 out tr' <-> exec st p2 out tr'.
+    fun p1 p2 => forall st out,
+        exec st p1 out <-> exec st p2 out.
 
   Arguments prog_equiv {T} _ _.
 
@@ -67,7 +67,6 @@ Ltac invert_exec :=
   Proof.
     split; intros.
     - repeat invert_exec; cleanup.
-      rewrite <- app_assoc.
       repeat econstructor; eauto.
 
       split_ors.
@@ -77,19 +76,35 @@ Ltac invert_exec :=
       econstructor; eauto.
       eapply ExecBindCrash; eauto.
       invert_exec.
-      rewrite <- app_assoc.
+      repeat econstructor; eauto.
+
+      split_ors.
+      invert_exec; cleanup.
+      split_ors; cleanup.
+      eapply ExecBindFail; auto.      
+      econstructor; eauto.
+      eapply ExecBindFail; eauto.
+      invert_exec.
       repeat econstructor; eauto.
     
     - repeat invert_exec; cleanup.
-      rewrite app_assoc.
       repeat (eapply ExecBind; eauto).
       
       split_ors.
-      repeat econstructor; eauto.
+      eapply ExecBindCrash; eauto.
+      eapply ExecBindCrash; eauto.
       invert_exec.
       split_ors.
       eapply ExecBindCrash; eauto.
       econstructor; eauto.
-      rewrite app_assoc.
+      repeat econstructor; eauto.
+
+      split_ors.
+      eapply ExecBindFail; eauto.
+      eapply ExecBindFail; eauto.
+      invert_exec.
+      split_ors.
+      eapply ExecBindFail; eauto.
+      econstructor; eauto.
       repeat econstructor; eauto.
   Qed.
