src/BlockAllocator.v
@@ -1,0 +1,1253 @@
+Require Import Primitives Omega Disk.
+Close Scope pred_scope.
+
+Axiom block_size: nat.
+Axiom block_size_eq: block_size = 64.
+
+Definition valid_bitlist l := length l = block_size /\ (forall i, In i l -> i < 2).
+Record bitlist :=
+  {
+   bits : list nat;                
+   valid : valid_bitlist bits
+  }.
+
+Fixpoint get_first_zero l :=
+  match l with
+  | nil => 0
+  | hd::tl =>
+    match hd with
+    | O => 0
+    | _ => S (get_first_zero tl)
+    end
+  end.
+
+Definition upd {T} i l (v: T) := firstn (length l) (firstn i l ++ v::skipn (S i) l).
+
+Theorem upd_valid_zero:
+  forall i l,
+    valid_bitlist l ->
+    valid_bitlist (upd i l 0).
+Proof. Admitted.
+
+Theorem upd_valid_one:
+  forall i l,
+    valid_bitlist l ->
+    valid_bitlist (upd i l 1).
+Proof. Admitted.
+
+Axiom value_to_bits: value -> bitlist.
+Axiom bits_to_value: bitlist -> value.
+Axiom value_to_bits_to_value : forall v, bits_to_value (value_to_bits v) = v.
+Axiom bits_to_value_to_bits : forall l, value_to_bits (bits_to_value l) = l.                                                                   
+Open Scope pred_scope.
+
+Definition rep (dh: @mem addr addr_dec value) : @pred addr addr_dec (set value) :=
+  fun d => (exists bitmap bl rest,
+    let bits := bits (value_to_bits bitmap) in
+    0 |-> (bitmap, bl) * rest *
+    [[forall i, nth i bits 0 = 0 -> dh i = None]] *
+    [[(forall i, nth i bits 0 = 1 -> exists vs, d (S i) = Some vs /\ dh i = Some (fst vs))%type]])%pred d.
+
+Definition alloc (v': value) : prog (option addr) :=
+  v <- Read 0;
+  let bits := bits (value_to_bits v) in
+  let valid := valid (value_to_bits v) in
+  let index := get_first_zero bits in
+  
+  if lt_dec index block_size then
+    _ <- Write (S index) v';
+    _ <- Write 0 (bits_to_value (Build_bitlist (upd index bits 1) (upd_valid_one index bits valid)));
+    Ret (Some index)
+  else
+    Ret None.
+
+Definition read a : prog (option value) :=
+  v <- Read 0;
+  let bits := bits (value_to_bits v) in
+  if lt_dec a block_size then
+    if addr_dec (nth a bits 0) 1 then
+      h <- Read a;
+      Ret (Some h)
+    else
+      Ret None
+  else
+    Ret None.
+
+Definition write a v' : prog (option unit) :=
+  v <- Read 0;
+  let bits := bits (value_to_bits v) in
+  if lt_dec a block_size then
+    if addr_dec (nth a bits 0) 1 then
+      _ <- Write a v';
+      Ret (Some tt)
+    else
+      Ret None
+  else
+    Ret None.
+
+Definition free a : prog unit :=
+  v <- Read 0;
+  let bits := bits (value_to_bits v) in
+  let valid := valid (value_to_bits v) in
+  if lt_dec a block_size then
+    if addr_dec (nth a bits 0) 1 then
+      Write 0 (bits_to_value (Build_bitlist (upd a bits 0) (upd_valid_zero a bits valid)))
+    else
+      Ret tt
+  else
+    Ret tt.
+
+(*
+Theorem hoare_triple_pre_ex':
+  forall T V (p: prog T) pre post crash,
+  (forall (v: V), hoare_triple (fun a => pre v a) p post crash) ->
+  hoare_triple (fun a => exists (v: V), pre v a) p post crash.
+Proof.
+  unfold hoare_triple; intros.
+  destruct_lift H0; cleanup.
+  eapply H; eauto.
+Qed.
+
+Theorem hoare_triple_pre_ex:
+  forall T V (p: prog T) pre post crash F,
+  (forall (v: V), hoare_triple (fun a => F * pre v a) p post crash) ->
+  hoare_triple (fun a => F * exists (v: V), pre v a) p post crash.
+Proof.
+  intros.
+  eapply hoare_triple_strengthen_pre.
+  apply hoare_triple_pre_ex'.
+  instantiate (1:= fun v a => F * pre v a).
+  simpl; eauto.
+  intros; cancel.
+Qed.
+
+Lemma upd_eq':
+  forall (A V : Type) (AEQ : EqDec A) (m : mem) (a : A) (v : V),
+    @upd _ _ AEQ m a v a = Some v.
+Proof.
+  intros; apply upd_eq; eauto.
+Qed.
+
+
+Theorem alloc_ok:
+  forall dh v,
+  << o >>
+   (rep dh)
+   (alloc v)
+  << o', r >>
+   (exists dh',
+    rep dh' *
+     [[(r = None /\ dh' = dh) \/
+       (exists a, r = Some a /\ dh' = upd dh a v)%type]])
+   (exists dh',
+    rep dh' *
+     [[(dh' = dh) \/
+       (exists h, dh' = upd dh h v)%type]]).
+Proof.
+  intros.
+  unfold alloc; simpl.
+  unfold rep.
+  repeat (apply hoare_triple_pre_ex; intros).
+
+  eapply hoare_triple_pimpl;
+  try solve [intros; simpl in *; eauto].
+  eapply hoare_triple_strengthen_pre;
+  [apply read_okay | intros; simpl; cancel].
+
+  intros; simpl.
+  destruct (addr_dec (value_to_nat r) 0); simpl.
+  {
+    intros; simpl. 
+    eapply hoare_triple_pimpl;
+    try solve [intros; simpl in *; eauto].
+    eapply hoare_triple_strengthen_pre;
+      [apply write_okay | intros; simpl; cancel].
+
+    intros; simpl.
+    destruct_pairs.
+    eapply hoare_triple_pimpl;
+    try solve [intros; simpl in *; eauto].
+    eapply hoare_triple_strengthen_pre;
+      [apply write_okay | intros; simpl; cancel].
+    {
+      intros; simpl.
+      eapply hoare_triple_strengthen_pre.
+      eapply hoare_triple_weaken_post_strong.
+      eapply hoare_triple_weaken_crash_strong.
+      apply ret_okay.  
+      3: intros; simpl; cancel.
+      
+      intros; simpl;
+        norm; [cancel|].
+      eassign (upd dh 1 v).
+      rewrite nat_to_value_to_nat; eauto.
+      rewrite upd_eq'.
+      repeat rewrite upd_ne; eauto.
+      destruct_lift H;        
+        destruct_lift H0; cleanup.
+      intuition (eauto; try omega).
+      rewrite upd_ne; eauto.
+      omega.
+
+      intros; simpl.
+      norm; [cancel|].
+      eassign (upd dh 1 v).
+      rewrite nat_to_value_to_nat; eauto.
+      rewrite upd_eq'.
+      repeat rewrite upd_ne; eauto.
+      destruct_lift H;
+        destruct_lift H0; cleanup.
+      intuition (eauto; try omega).
+      rewrite upd_ne; eauto.
+      omega.
+    }
+    
+    all: intros; simpl in *;
+      destruct_lift H;
+      destruct_lift H0; cleanup;
+        cancel; eauto.
+  }
+  destruct (addr_dec (value_to_nat r) 1); simpl.
+  {
+    intros; simpl. 
+    eapply hoare_triple_pimpl;
+    try solve [intros; simpl in *; eauto].
+    eapply hoare_triple_strengthen_pre;
+      [apply write_okay | intros; simpl; cancel].
+
+    intros; simpl.
+    destruct_pairs.
+    eapply hoare_triple_pimpl;
+    try solve [intros; simpl in *; eauto].
+    eapply hoare_triple_strengthen_pre;
+    [apply write_okay | intros; simpl; cancel].
+
+    {
+      intros; simpl.
+      eapply hoare_triple_strengthen_pre.
+      eapply hoare_triple_weaken_post_strong.
+      eapply hoare_triple_weaken_crash_strong.
+      apply ret_okay.  
+      3: intros; simpl; cancel.
+      
+      intros; simpl;
+        norm; [cancel|].
+      eassign (upd dh 2 v).
+      rewrite nat_to_value_to_nat; eauto.
+      rewrite upd_eq'.
+      repeat rewrite upd_ne; eauto.
+      destruct_lift H;
+        destruct_lift H0; cleanup.
+      intuition (eauto; try omega).
+      rewrite upd_ne; eauto.
+      omega.
+
+      intros; simpl.
+      norm; [cancel|].
+      eassign (upd dh 2 v).
+      rewrite nat_to_value_to_nat; eauto.
+      rewrite upd_eq'.
+      repeat rewrite upd_ne; eauto.
+      destruct_lift H;
+        destruct_lift H0; cleanup.
+      intuition (eauto; try omega).
+      rewrite upd_ne; eauto.
+      omega.
+    }
+    all: try solve [
+      intros; simpl in *;
+      destruct_lift H;
+        destruct_lift H0; cleanup;
+      cancel; eauto].      
+  }
+  destruct (addr_dec (value_to_nat r) 2); simpl.
+  {
+    intros; simpl. 
+    eapply hoare_triple_pimpl;
+    try solve [intros; simpl in *; eauto].
+    eapply hoare_triple_strengthen_pre;
+    [apply write_okay | intros; simpl; cancel].
+    
+    intros; simpl.
+    destruct_pairs.
+    eapply hoare_triple_pimpl;
+    try solve [intros; simpl in *; eauto].
+    eapply hoare_triple_strengthen_pre;
+    [apply write_okay | intros; simpl; cancel].
+
+    {
+      intros; simpl.
+      eapply hoare_triple_strengthen_pre.
+      eapply hoare_triple_weaken_post_strong.
+      eapply hoare_triple_weaken_crash_strong.
+      apply ret_okay.  
+      3: intros; simpl; cancel.
+      
+      intros; simpl;
+        norm; [cancel|].
+      eassign (upd dh 1 v).
+      rewrite nat_to_value_to_nat; eauto.
+      rewrite upd_eq'.
+      repeat rewrite upd_ne; eauto.
+      destruct_lift H;
+        destruct_lift H0; cleanup.
+      intuition (eauto; try omega).
+      rewrite upd_ne; eauto.
+      omega.
+
+      intros; simpl.
+      norm; [cancel|].
+      eassign (upd dh 1 v).
+      rewrite nat_to_value_to_nat; eauto.
+      rewrite upd_eq'.
+      repeat rewrite upd_ne; eauto.
+      destruct_lift H;
+        destruct_lift H0; cleanup.
+      intuition (eauto; try omega).
+      rewrite upd_ne; eauto.
+      omega.
+    }
+    all: try solve [
+      intros; simpl in *;
+      destruct_lift H;
+        destruct_lift H0; cleanup;
+        norm; [cancel| intuition (eauto; try omega)]
+      ].
+  }
+
+  {
+      intros; simpl.
+      eapply hoare_triple_strengthen_pre.
+      eapply hoare_triple_weaken_post_strong.
+      eapply hoare_triple_weaken_crash_strong.
+      apply ret_okay.
+      3: intros; simpl; rewrite emp_star_r; eauto.
+      
+      intros; simpl; destruct_lift H; cleanup.
+      norm; [cancel| intuition (eauto; try omega)].
+
+      intros; simpl; destruct_lift H; cleanup.
+      norm; [cancel| intuition (eauto; try omega)].
+  }
+
+  all: try solve [
+       intros; simpl; destruct_lift H; cleanup;
+       norm; [cancel| intuition (eauto; try omega)]
+           ].
+Qed.
+
+Theorem read_ok:
+  forall a dh,
+  << o >>
+   (rep dh)
+   (read a)
+  << o', r >>
+   (rep dh *
+     [[(r = None /\ (dh a = None \/ a = 0 \/ a > 2)) \/
+       (exists v, r = Some v /\ dh a = Some v)%type]])
+   (rep dh).
+Proof.
+  intros.
+  unfold read; simpl.
+
+  unfold rep.
+  repeat (apply hoare_triple_pre_ex; intros).
+  
+  eapply hoare_triple_pimpl;
+    try solve [intros; simpl in *; eauto].
+  eapply hoare_triple_strengthen_pre;
+    [apply read_okay | intros; simpl; cancel].
+
+  simpl. destruct (addr_dec a 1); subst.
+  {
+    intros; simpl.
+    destruct (addr_dec (value_to_nat r) 1); simpl.
+    {
+    eapply hoare_triple_pimpl;
+    try solve [intros; simpl in *; eauto].
+    eapply hoare_triple_strengthen_pre;
+    [apply read_okay | intros; simpl; cancel].
+
+    {
+      intros; simpl.
+      eapply hoare_triple_weaken_post_weak.
+      eapply hoare_triple_weaken_crash_strong.
+      eapply hoare_triple_strengthen_pre.
+      apply ret_okay.
+      
+      intros; simpl in *.
+      destruct_lift H;
+        destruct_lift H0; cleanup;
+          cancel; eauto.
+      
+      intros; simpl in *.
+      destruct_lift H;
+        destruct_lift H0; cleanup;
+          cancel; eauto.
+
+      intros; simpl in *.
+      destruct_lift H;
+        destruct_lift H0;
+        destruct_lift H1;
+        cleanup;
+          cancel; eauto.
+    }
+    intros; simpl in *;
+      destruct_lift H;
+      destruct_lift H0; cleanup;
+        norm; [cancel| intuition (eauto; try omega)].
+    }
+
+    destruct (addr_dec (value_to_nat r) 3); simpl.
+    {
+    eapply hoare_triple_pimpl;
+    try solve [intros; simpl in *; eauto].
+    eapply hoare_triple_strengthen_pre;
+    [apply read_okay | intros; simpl; cancel].
+
+    {
+      intros; simpl.
+      eapply hoare_triple_weaken_post_weak.
+      eapply hoare_triple_weaken_crash_strong.
+      eapply hoare_triple_strengthen_pre.
+      apply ret_okay.
+      
+      intros; simpl in *.
+      destruct_lift H;
+        destruct_lift H0; cleanup;
+          cancel; eauto.
+      
+      intros; simpl in *.
+      destruct_lift H;
+        destruct_lift H0; cleanup;
+          cancel; eauto.
+
+      intros; simpl in *.
+      destruct_lift H;
+        destruct_lift H0;
+        destruct_lift H1;
+        cleanup;
+          cancel; eauto.
+    }
+    intros; simpl in *;
+      destruct_lift H;
+      destruct_lift H0; cleanup;
+        norm; [cancel| intuition (eauto; try omega)].
+    }
+
+      {
+      intros; simpl.
+      eapply hoare_triple_weaken_post_weak.
+      eapply hoare_triple_weaken_crash_strong.
+      eapply hoare_triple_strengthen_pre.
+      apply ret_okay.
+
+      eassign (F * rep dh * ⟦⟦ r = v ⟧⟧).
+      destruct_lift H;
+        cleanup.
+      intros; simpl in *; unfold rep; cancel.
+      
+      unfold rep; intros; simpl in *.
+      destruct_lift H; cleanup.
+      norm; [cancel| intuition (eauto; try omega)].
+      
+
+      intros; simpl in *.
+      unfold rep;
+      destruct_lift H; cleanup;
+      norm; [cancel| intuition (eauto; try omega)].
+      
+      left; split; eauto.
+      left.
+      destruct (addr_dec (value_to_nat v) 0).
+      destruct H8; eauto.
+      destruct (addr_dec (value_to_nat v) 2);
+        destruct H6; eauto.
+      omega.
+    }
+  }
+  
+
+  destruct (addr_dec a 2); subst.
+  {
+    intros; simpl.
+    destruct (addr_dec (value_to_nat r) 2); simpl.
+    {
+    eapply hoare_triple_pimpl;
+    try solve [intros; simpl in *; eauto].
+    eapply hoare_triple_strengthen_pre;
+    [apply read_okay | intros; simpl; cancel].
+
+    {
+      intros; simpl.
+      eapply hoare_triple_weaken_post_weak.
+      eapply hoare_triple_weaken_crash_strong.
+      eapply hoare_triple_strengthen_pre.
+      apply ret_okay.
+      
+      intros; simpl in *.
+      destruct_lift H;
+        destruct_lift H0; cleanup;
+          cancel; eauto.
+      
+      intros; simpl in *.
+      destruct_lift H;
+        destruct_lift H0; cleanup;
+          cancel; eauto.
+
+      intros; simpl in *.
+      destruct_lift H;
+        destruct_lift H0;
+        destruct_lift H1;
+        cleanup;
+          cancel; eauto.
+    }
+    intros; simpl in *;
+      destruct_lift H;
+      destruct_lift H0; cleanup;
+        norm; [cancel| intuition (eauto; try omega)].
+    }
+
+    destruct (addr_dec (value_to_nat r) 3); simpl.
+    {
+    eapply hoare_triple_pimpl;
+    try solve [intros; simpl in *; eauto].
+    eapply hoare_triple_strengthen_pre;
+    [apply read_okay | intros; simpl; cancel].
+
+    {
+      intros; simpl.
+      eapply hoare_triple_weaken_post_weak.
+      eapply hoare_triple_weaken_crash_strong.
+      eapply hoare_triple_strengthen_pre.
+      apply ret_okay.
+      
+      intros; simpl in *.
+      destruct_lift H;
+        destruct_lift H0; cleanup;
+          cancel; eauto.
+      
+      intros; simpl in *.
+      destruct_lift H;
+        destruct_lift H0; cleanup;
+          cancel; eauto.
+
+      intros; simpl in *.
+      destruct_lift H;
+        destruct_lift H0;
+        destruct_lift H1;
+        cleanup;
+          cancel; eauto.
+    }
+    intros; simpl in *;
+      destruct_lift H;
+      destruct_lift H0; cleanup;
+        norm; [cancel| intuition (eauto; try omega)].
+    }
+
+      {
+      intros; simpl.
+      eapply hoare_triple_weaken_post_weak.
+      eapply hoare_triple_weaken_crash_strong.
+      eapply hoare_triple_strengthen_pre.
+      apply ret_okay.
+
+      eassign (F * rep dh * ⟦⟦ r = v ⟧⟧).
+      destruct_lift H;
+        cleanup.
+      intros; simpl in *; unfold rep; cancel.
+      
+      unfold rep; intros; simpl in *.
+      destruct_lift H;
+        cleanup.
+      norm; [cancel| intuition (eauto; try omega)].      
+
+      intros; simpl in *.
+      unfold rep;
+      destruct_lift H;
+        destruct_lift H0;
+        cleanup;
+      norm; [cancel| intuition (eauto; try omega)].
+      
+      left; split; eauto.
+      left.
+      destruct (addr_dec (value_to_nat v) 0).
+      destruct H8; eauto.
+      destruct (addr_dec (value_to_nat v) 1).
+      destruct H7; eauto.
+      omega.
+    }
+  }
+
+  {
+      intros; simpl.
+      eapply hoare_triple_weaken_post_weak.
+      eapply hoare_triple_weaken_crash_strong.
+      eapply hoare_triple_strengthen_pre.
+      apply ret_okay.
+      intros; simpl; rewrite emp_star_r; eauto.
+      destruct_lift H; cancel.
+      destruct_lift H; cancel.
+      left; intuition.      
+      right; omega.
+  }
+
+  intros; simpl.
+  destruct_lift H; cancel.
+Qed.
+
+Lemma exis_lift_absorb:
+  forall A AEQ V T (P: T -> @pred A AEQ V) Q,
+    (exists x, P x) * [[ Q ]] =p=> exists x, (P x * [[Q]]).
+Proof.
+  intros; cancel.
+Qed.
+
+
+Theorem write_ok:
+  forall dh a v,
+  << o >>
+   (rep dh)
+   (write a v)
+  << o', r >>
+   (exists dh',
+    rep dh' *
+     [[(r = None /\ dh' = dh) \/
+       (r = Some tt /\ dh a <> None /\ dh' = upd dh a v)%type]])
+   (exists dh',
+    rep dh' *
+     [[(dh' = dh \/ (dh a <> None /\ dh' = upd dh a v))%type]]).
+Proof.
+  intros.
+  unfold write; simpl.
+
+  repeat (apply hoare_triple_pre_ex; intros).
+    eapply hoare_triple_pimpl;
+      try solve [intros; simpl in *; eauto].
+    eapply hoare_triple_strengthen_pre;
+      [apply read_okay | intros; simpl; cancel].
+    
+  intros; simpl; destruct (addr_dec a 1); subst.
+  {
+    intros; simpl.
+    destruct (addr_dec (value_to_nat r) 1); simpl.
+    {
+      eapply hoare_triple_pimpl;
+        try solve [intros; simpl in *; eauto].
+      eapply hoare_triple_strengthen_pre;
+        [apply write_okay | intros; simpl; cancel].
+      
+      {
+        intros; simpl.
+        eapply hoare_triple_weaken_post_weak.
+        eapply hoare_triple_weaken_crash_strong.
+        eapply hoare_triple_strengthen_pre.
+        apply ret_okay.
+        
+        intros; simpl in *.
+        rewrite <- emp_star_r; eauto.
+        
+        intros; unfold rep; simpl in *.
+        norm; [cancel|].
+        eassign (upd dh 1 v).
+        rewrite upd_eq'.
+        repeat rewrite upd_ne; eauto.
+        destruct_lift H;
+          destruct_lift H0;
+          cleanup;
+          intuition (eauto; try omega).
+        rewrite upd_ne; eauto; omega.
+        right; intuition eauto.
+        cleanup.
+
+        intros; unfold rep; simpl in *.
+        norm; [cancel|].
+        eassign (upd dh 1 v).
+        rewrite upd_eq'.
+        repeat rewrite upd_ne; eauto.
+        destruct_lift H;
+          destruct_lift H0;
+          cleanup;
+          intuition (eauto; try omega).
+        rewrite upd_ne; eauto; omega.
+        right; intuition eauto.
+        cleanup.
+      }        
+      intros; unfold rep; simpl in *.
+      destruct_lift H;
+          destruct_lift H0;
+          cleanup;
+        norm; [cancel| intuition (eauto; try omega)].
+    }
+
+    destruct (addr_dec (value_to_nat r) 3); simpl.
+    {
+      eapply hoare_triple_pimpl;
+        try solve [intros; simpl in *; eauto].
+      eapply hoare_triple_strengthen_pre;
+        [apply write_okay | intros; simpl; cancel].
+      {
+        intros; simpl.
+        eapply hoare_triple_weaken_post_weak.
+        eapply hoare_triple_weaken_crash_strong.
+        eapply hoare_triple_strengthen_pre.
+        apply ret_okay.
+        
+        intros; simpl in *.
+        rewrite <- emp_star_r; eauto.
+        
+        intros; unfold rep; simpl in *.
+        norm; [cancel|].
+        eassign (upd dh 1 v).
+        rewrite upd_eq'.
+        repeat rewrite upd_ne; eauto.
+        destruct_lift H;
+          destruct_lift H0;
+          cleanup;
+          intuition (eauto; try omega).
+        rewrite upd_ne; eauto; omega.
+        right; intuition eauto.
+        cleanup.
+
+        intros; unfold rep; simpl in *.
+        norm; [cancel|].
+        eassign (upd dh 1 v).
+        rewrite upd_eq'.
+        repeat rewrite upd_ne; eauto.
+        destruct_lift H;
+          destruct_lift H0;
+          cleanup;
+          intuition (eauto; try omega).
+        rewrite upd_ne; eauto; omega.
+        right; intuition eauto.
+        cleanup.
+      }        
+      intros; unfold rep; simpl in *.
+      destruct_lift H;
+          destruct_lift H0;
+          cleanup;
+        norm; [cancel| intuition (eauto; try omega)].
+    }
+
+      {
+      intros; simpl.
+      eapply hoare_triple_weaken_post_weak.
+      eapply hoare_triple_weaken_crash_strong.
+      eapply hoare_triple_strengthen_pre.
+      apply ret_okay.
+
+      eassign (F * rep dh).
+      destruct_lift H;
+        cleanup.
+      intros; simpl in *; unfold rep; cancel.
+
+      cancel.
+      cancel.
+    }
+  }
+  
+
+  destruct (addr_dec a 2); subst.
+   {
+    intros; simpl.
+    destruct (addr_dec (value_to_nat r) 2); simpl.
+    {
+      eapply hoare_triple_pimpl;
+        try solve [intros; simpl in *; eauto].
+      eapply hoare_triple_strengthen_pre;
+        [apply write_okay | intros; simpl; cancel].
+      destruct_lift H; cleanup.
+      
+      {
+        intros; simpl.
+        eapply hoare_triple_weaken_post_weak.
+        eapply hoare_triple_weaken_crash_strong.
+        eapply hoare_triple_strengthen_pre.
+        apply ret_okay.
+
+        intros; simpl in *.
+        rewrite <- emp_star_r; eauto.
+        
+        intros; unfold rep; simpl in *.
+        norm; [cancel|].
+        eassign (upd dh 2 v).
+        rewrite upd_eq'.
+        repeat rewrite upd_ne; eauto.
+        destruct_lift H;
+          destruct_lift H0;
+          cleanup;
+          intuition (eauto; try omega).
+        rewrite upd_ne; eauto; omega.
+        right; intuition eauto.
+        cleanup.
+
+        intros; unfold rep; simpl in *.
+        norm; [cancel|].
+        eassign (upd dh 2 v).
+        rewrite upd_eq'.
+        repeat rewrite upd_ne; eauto.
+        destruct_lift H;
+          destruct_lift H0;
+          cleanup;
+          intuition (eauto; try omega).
+        rewrite upd_ne; eauto; omega.
+        right; intuition eauto.
+        cleanup.
+      }        
+      intros; unfold rep; simpl in *.
+      destruct_lift H;
+          destruct_lift H0;
+          cleanup;
+        norm; [cancel| intuition (eauto; try omega)].
+    }
+
+    destruct (addr_dec (value_to_nat r) 3); simpl.
+    {
+      eapply hoare_triple_pimpl;
+        try solve [intros; simpl in *; eauto].
+      eapply hoare_triple_strengthen_pre;
+        [apply write_okay | intros; simpl; cancel].
+      {
+        intros; simpl.
+        eapply hoare_triple_weaken_post_weak.
+        eapply hoare_triple_weaken_crash_strong.
+        eapply hoare_triple_strengthen_pre.
+        apply ret_okay.
+        
+        intros; simpl in *.
+        rewrite <- emp_star_r; eauto.
+        
+        intros; unfold rep; simpl in *.
+        norm; [cancel|].
+        eassign (upd dh 2 v).
+        rewrite upd_eq'.
+        repeat rewrite upd_ne; eauto.
+        destruct_lift H;
+          destruct_lift H0;
+          cleanup;
+          intuition (eauto; try omega).
+        rewrite upd_ne; eauto; omega.
+        right; intuition eauto.
+        cleanup.
+
+        intros; unfold rep; simpl in *.
+        norm; [cancel|].
+        eassign (upd dh 2 v).
+        rewrite upd_eq'.
+        repeat rewrite upd_ne; eauto.
+        destruct_lift H;
+          destruct_lift H0;
+          cleanup;
+          intuition (eauto; try omega).
+        rewrite upd_ne; eauto; omega.
+        right; intuition eauto.
+        cleanup.
+      }        
+      intros; unfold rep; simpl in *.
+      destruct_lift H;
+          destruct_lift H0;
+          cleanup;
+        norm; [cancel| intuition (eauto; try omega)].
+    }
+
+      {
+      intros; simpl.
+      eapply hoare_triple_weaken_post_weak.
+      eapply hoare_triple_weaken_crash_strong.
+      eapply hoare_triple_strengthen_pre.
+      apply ret_okay.
+
+      eassign (F * rep dh).
+      destruct_lift H;
+        cleanup.
+      intros; simpl in *; unfold rep; cancel.
+
+      cancel.
+      cancel.
+
+      }
+   }
+
+   {
+      intros; simpl.
+      eapply hoare_triple_weaken_post_weak.
+      eapply hoare_triple_weaken_crash_strong.
+      eapply hoare_triple_strengthen_pre.
+      apply ret_okay.
+
+      eassign (F * rep dh).
+      destruct_lift H;
+        cleanup.
+      intros; simpl in *; unfold rep; cancel.
+      
+      all: cancel.
+   }
+   intros; simpl in *;
+     destruct_lift H; cleanup.
+   cancel; unfold rep; cancel.
+Qed.
+
+Lemma delete_eq:
+  forall A AEQ V (m: @mem A AEQ V) a,
+    delete m a a = None.
+Proof.
+  intros; unfold delete; simpl.
+  destruct (AEQ a a); intuition.
+Qed.
+
+Lemma delete_ne:
+  forall A AEQ V (m: @mem A AEQ V) a a',
+    a <> a' ->
+    delete m a a' = m a'.
+Proof.
+  intros; unfold delete; simpl.
+  destruct (AEQ a' a); subst; intuition.
+Qed.
+        
+
+Theorem free_ok:
+  forall dh a,
+  << o >>
+   (rep dh)
+   (free a)
+  << o', r >>
+   (rep (delete dh a))
+   (rep (delete dh a)).
+Proof.
+  intros.
+  unfold free; simpl.
+
+  destruct (addr_dec a 1); subst.
+  {
+    
+
+    intros; simpl.
+    eapply hoare_triple_pimpl;
+      try solve [intros; simpl in *; eauto].
+    eapply hoare_triple_strengthen_pre;
+      [apply unseal_okay | intros; simpl; cancel].
+    apply upd_eq; eauto.
+    simpl; apply can_access_public.
+
+    intros; simpl.
+    destruct (addr_dec (value_to_nat r0) 1); simpl.
+    {
+      eapply hoare_triple_pimpl;
+        try solve [intros; simpl in *; eauto].
+      eapply hoare_triple_strengthen_pre;
+        [apply seal_okay | intros; simpl; cancel].
+    
+      {
+        intros; simpl.
+        eapply hoare_triple_weaken_post_weak.
+        eapply hoare_triple_weaken_crash_strong.
+        eapply hoare_triple_strengthen_pre.
+        apply write_okay.
+        
+        intros; simpl in *.
+        cancel.
+        apply upd_eq'.
+        
+        intros; simpl in *.
+        norm; [cancel|].
+        eassign dh.
+        destruct_lift H;
+          destruct_lift H0;
+          destruct_lift H1;
+          cleanup;
+          intuition (eauto; try omega).
+
+        intros; simpl in *.
+        norm; [cancel|].
+        rewrite delete_eq.
+        repeat rewrite delete_ne; eauto.
+        rewrite nat_to_value_to_nat.
+        destruct_lift H;
+          destruct_lift H0;
+          destruct_lift H1;
+          cleanup;
+          intuition (eauto; try omega).
+        rewrite delete_ne; eauto; omega.
+      }        
+      intros; simpl in *.
+      destruct_lift H;
+          destruct_lift H0;
+          destruct_lift H1;
+          cleanup;
+        norm; [cancel| intuition (eauto; try omega)].
+    }
+
+    destruct (addr_dec (value_to_nat r0) 3); simpl.
+    {
+      eapply hoare_triple_pimpl;
+        try solve [intros; simpl in *; eauto].
+      eapply hoare_triple_strengthen_pre;
+        [apply seal_okay | intros; simpl; cancel].
+    
+      {
+        intros; simpl.
+        eapply hoare_triple_weaken_post_weak.
+        eapply hoare_triple_weaken_crash_strong.
+        eapply hoare_triple_strengthen_pre.
+        apply write_okay.
+        
+        intros; simpl in *.
+        cancel.
+        apply upd_eq'.
+        
+        intros; simpl in *.
+        norm; [cancel|].
+        eassign dh.
+        destruct_lift H;
+          destruct_lift H0;
+          destruct_lift H1;
+          cleanup;
+          intuition (eauto; try omega).
+
+        intros; simpl in *.
+        norm; [cancel|].
+        rewrite delete_eq.
+        repeat rewrite delete_ne; eauto.
+        rewrite nat_to_value_to_nat.
+        destruct_lift H;
+          destruct_lift H0;
+          destruct_lift H1;
+          cleanup;
+          intuition (eauto; try omega).
+        rewrite delete_ne; eauto; omega.
+      }        
+      intros; simpl in *.
+      destruct_lift H;
+          destruct_lift H0;
+          destruct_lift H1;
+          cleanup;
+        norm; [cancel| intuition (eauto; try omega)].
+    }
+
+    {
+      {
+        intros; simpl.
+        eapply hoare_triple_weaken_post_weak.
+        eapply hoare_triple_weaken_crash_strong.
+        eapply hoare_triple_strengthen_pre.
+        apply ret_okay.
+        
+        intros; simpl in *.
+        eassign (((((0 |-> (Public, v, v0) ✶ F) ✶ 1 |-> v1) ✶ 2 |-> v2) ✶ (⟦⟦ r0 = v ⟧⟧))).
+        cancel.
+        
+        intros; simpl in *.
+        norm; [cancel|].
+        eassign dh.
+        destruct_lift H;
+          destruct_lift H0;
+          cleanup;
+          intuition (eauto; try omega).
+
+        intros; simpl in *.
+        norm; [cancel|].
+        rewrite delete_eq.
+        repeat rewrite delete_ne; eauto.
+        destruct_lift H;
+          destruct_lift H0;
+          destruct_lift H1;
+          cleanup;
+          intuition (eauto; try omega).
+        rewrite delete_ne; eauto; omega.
+      }
+    }
+    
+      intros; simpl in *;
+      destruct_lift H;
+          destruct_lift H0;
+          cleanup;
+          norm; [cancel| intuition (eauto; try omega)].
+    intros; simpl in *;
+      destruct_lift H;
+          cleanup;
+        norm; [cancel| intuition (eauto; try omega)].
+  }
+
+  destruct (addr_dec a 2); subst.
+  {
+    unfold rep.
+    repeat (apply hoare_triple_pre_ex; intros).
+    eapply hoare_triple_pimpl;
+      try solve [intros; simpl in *; eauto].
+    eapply hoare_triple_strengthen_pre;
+      [apply read_okay | intros; simpl; cancel].
+
+    intros; simpl.
+    eapply hoare_triple_pimpl;
+      try solve [intros; simpl in *; eauto].
+    eapply hoare_triple_strengthen_pre;
+      [apply unseal_okay | intros; simpl; cancel].
+    apply upd_eq; eauto.
+    simpl; apply can_access_public.
+
+    intros; simpl.
+    destruct (addr_dec (value_to_nat r0) 2); simpl.
+    {
+      eapply hoare_triple_pimpl;
+        try solve [intros; simpl in *; eauto].
+      eapply hoare_triple_strengthen_pre;
+        [apply seal_okay | intros; simpl; cancel].
+    
+      {
+        intros; simpl.
+        eapply hoare_triple_weaken_post_weak.
+        eapply hoare_triple_weaken_crash_strong.
+        eapply hoare_triple_strengthen_pre.
+        apply write_okay.
+        
+        intros; simpl in *.
+        cancel.
+        apply upd_eq'.
+        
+        intros; simpl in *.
+        norm; [cancel|].
+        eassign dh.
+        destruct_lift H;
+          destruct_lift H0;
+          destruct_lift H1;
+          cleanup;
+          intuition (eauto; try omega).
+
+        intros; simpl in *.
+        norm; [cancel|].
+        rewrite delete_eq.
+        repeat rewrite delete_ne; eauto.
+        rewrite nat_to_value_to_nat.
+        destruct_lift H;
+          destruct_lift H0;
+          destruct_lift H1;
+          cleanup;
+          intuition (eauto; try omega).
+        rewrite delete_ne; eauto; omega.
+      }        
+      intros; simpl in *.
+      destruct_lift H;
+          destruct_lift H0;
+          destruct_lift H1;
+          cleanup;
+        norm; [cancel| intuition (eauto; try omega)].
+    }
+
+    destruct (addr_dec (value_to_nat r0) 3); simpl.
+    {
+      eapply hoare_triple_pimpl;
+        try solve [intros; simpl in *; eauto].
+      eapply hoare_triple_strengthen_pre;
+        [apply seal_okay | intros; simpl; cancel].
+    
+      {
+        intros; simpl.
+        eapply hoare_triple_weaken_post_weak.
+        eapply hoare_triple_weaken_crash_strong.
+        eapply hoare_triple_strengthen_pre.
+        apply write_okay.
+        
+        intros; simpl in *.
+        cancel.
+        apply upd_eq'.
+        
+        intros; simpl in *.
+        norm; [cancel|].
+        eassign dh.
+        destruct_lift H;
+          destruct_lift H0;
+          destruct_lift H1;
+          cleanup;
+          intuition (eauto; try omega).
+
+        intros; simpl in *.
+        norm; [cancel|].
+        rewrite delete_eq.
+        repeat rewrite delete_ne; eauto.
+        rewrite nat_to_value_to_nat.
+        destruct_lift H;
+          destruct_lift H0;
+          destruct_lift H1;
+          cleanup;
+          intuition (eauto; try omega).
+        rewrite delete_ne; eauto; omega.
+      }        
+      intros; simpl in *.
+      destruct_lift H;
+          destruct_lift H0;
+          destruct_lift H1;
+          cleanup;
+        norm; [cancel| intuition (eauto; try omega)].
+    }
+
+    {
+      {
+        intros; simpl.
+        eapply hoare_triple_weaken_post_weak.
+        eapply hoare_triple_weaken_crash_strong.
+        eapply hoare_triple_strengthen_pre.
+        apply ret_okay.
+        
+        intros; simpl in *.
+        eassign (((((0 |-> (Public, v, v0) ✶ F) ✶ 1 |-> v1) ✶ 2 |-> v2) ✶ (⟦⟦ r0 = v ⟧⟧))).
+        cancel.
+        
+        intros; simpl in *.
+        norm; [cancel|].
+        eassign dh.
+        destruct_lift H;
+          destruct_lift H0;
+          cleanup;
+          intuition (eauto; try omega).
+
+        intros; simpl in *.
+        norm; [cancel|].
+        rewrite delete_eq.
+        repeat rewrite delete_ne; eauto.
+        destruct_lift H;
+          destruct_lift H0;
+          destruct_lift H1;
+          cleanup;
+          intuition (eauto; try omega).
+        rewrite delete_ne; eauto; omega.
+      }
+    }
+    
+      intros; simpl in *;
+      destruct_lift H;
+          destruct_lift H0;
+          cleanup;
+          norm; [cancel| intuition (eauto; try omega)].
+    intros; simpl in *;
+      destruct_lift H;
+          cleanup;
+        norm; [cancel| intuition (eauto; try omega)].
+  }
+
+
+  {
+    intros; simpl.
+    eapply hoare_triple_weaken_post_weak.
+    eapply hoare_triple_weaken_crash_strong.
+    eapply hoare_triple_strengthen_pre.
+    apply ret_okay.
+
+    all: cancel.
+    cancel.
+    unfold rep.
+    destruct a.
+    unfold delete at 1.
+    destruct (addr_dec 0 0); intuition.
+    repeat rewrite delete_ne; eauto.
+    cancel.
+    rewrite delete_ne; eauto.
+    omega.
+
+    repeat rewrite delete_ne; eauto.
+    cancel.
+    destruct (addr_dec (S a) n1); subst.
+    apply delete_eq.
+    rewrite delete_ne; eauto.
+  }
+Qed.
+*)
