src/DestructVarname.v
@@ -14,7 +14,7 @@ Ltac clear_varname :=
 
 Ltac destruct_prod :=
   match goal with
-  | [ v: valueset |- _ ] =>
+  | [ v: set _ |- _ ] =>
     let v0 := fresh v "_cur" in
     let v1 := fresh v "_old" in
     destruct v as [v0 v1]
@@ -130,21 +130,6 @@ Ltac destruct_varname4 :=
 		end
 	end.
 
-Theorem destruct_varname6 : forall XN1 X1 XN2 X2 XN3 X3 XN4 X4 XN5 X5 XN6 X6 X7 
-				(p : (XN1 * X1) * ((XN2 * X2) * ((XN3 * X3) * ((XN4 * X4) * ((XN5 * X5) * ((XN6 * X6) * X7)))))),
-	exists xn1 x1 xn2 x2 xn3 x3 xn4 x4 xn5 x5 xn6 x6 x7, p = ((xn1, x1), ((xn2, x2), ((xn3, x3), ((xn4, x4), ((xn5, x5), ((xn6, x6), x7)))))).
-Proof. intros. repeat destruct_prod. repeat eexists. Qed.
-
-Ltac destruct_varname6 :=
-	match goal with
-	| [ H : VARNAME (_) * _ * (VARNAME (_) * _ * (VARNAME (_) * _ * (VARNAME (_) * _ * (VARNAME (_) * _ * ((VARNAME (_) * _) * _))))) |- _ ] =>
-		let Hx := fresh in
-		pose proof (destruct_varname6 H) as Hx;
-		match type of Hx with
-		| exists (_ : VARNAME (vn1)) _ (_ : VARNAME (vn2)) _ (_ : VARNAME (vn3)) _ (_ : VARNAME (vn4)) _ (_ : VARNAME (vn5)) _ (_ : VARNAME (vn6)) _ _ , _ = _ =>
-			destruct Hx as [? [?vn1 [? [?vn2 [? [?vn3 [? [?vn4 [? [?vn5 [? [?vn6 [? Hx] ] ] ] ] ] ] ] ] ] ] ] ]
-		end
-	end.
 
 Theorem destruct_varname8 : forall XN1 X1 XN2 X2 XN3 X3 XN4 X4 XN5 X5 XN6 X6 XN7 X7 XN8 X8 X9 
 				(p : (XN1 * X1) * ((XN2 * X2) * ((XN3 * X3) * ((XN4 * X4) * ((XN5 * X5) * ((XN6 * X6) * ((XN7 * X7) * ((XN8 * X8) * X9)))))))),
@@ -162,53 +147,6 @@ Ltac destruct_varname8 :=
 		end
 	end.
 
-Theorem destruct_varname10 : forall XN1 X1 XN2 X2 XN3 X3 XN4 X4 XN5 X5 XN6 X6 XN7 X7 XN8 X8 XN9 X9 XN10 X10 X11 
-				(p : (XN1 * X1) * ((XN2 * X2) * ((XN3 * X3) * ((XN4 * X4) * ((XN5 * X5) * ((XN6 * X6) * ((XN7 * X7) * ((XN8 * X8) * ((XN9 * X9) * ((XN10 * X10) * X11)))))))))),
-	exists xn1 x1 xn2 x2 xn3 x3 xn4 x4 xn5 x5 xn6 x6 xn7 x7 xn8 x8 xn9 x9 xn10 x10 x11, p = ((xn1, x1), ((xn2, x2), ((xn3, x3), ((xn4, x4), ((xn5, x5), ((xn6, x6), ((xn7, x7), ((xn8, x8), ((xn9, x9), ((xn10, x10), x11)))))))))).
-Proof. intros. repeat destruct_prod. repeat eexists. Qed.
-
-Ltac destruct_varname10 :=
-	match goal with
-	| [ H : VARNAME (_) * _ * (VARNAME (_) * _ * (VARNAME (_) * _ * (VARNAME (_) * _ * (VARNAME (_) * _ * (VARNAME (_) * _ * (VARNAME (_) * _ * (VARNAME (_) * _ * (VARNAME (_) * _ * ((VARNAME (_) * _) * _))))))))) |- _ ] =>
-		let Hx := fresh in
-		pose proof (destruct_varname10 H) as Hx;
-		match type of Hx with
-		| exists (_ : VARNAME (vn1)) _ (_ : VARNAME (vn2)) _ (_ : VARNAME (vn3)) _ (_ : VARNAME (vn4)) _ (_ : VARNAME (vn5)) _ (_ : VARNAME (vn6)) _ (_ : VARNAME (vn7)) _ (_ : VARNAME (vn8)) _ (_ : VARNAME (vn9)) _ (_ : VARNAME (vn10)) _ _ , _ = _ =>
-			destruct Hx as [? [?vn1 [? [?vn2 [? [?vn3 [? [?vn4 [? [?vn5 [? [?vn6 [? [?vn7 [? [?vn8 [? [?vn9 [? [?vn10 [? Hx] ] ] ] ] ] ] ] ] ] ] ] ] ] ] ] ] ] ] ] ]
-		end
-	end.
-
-Theorem destruct_varname12 : forall XN1 X1 XN2 X2 XN3 X3 XN4 X4 XN5 X5 XN6 X6 XN7 X7 XN8 X8 XN9 X9 XN10 X10 XN11 X11 XN12 X12 X13 
-				(p : (XN1 * X1) * ((XN2 * X2) * ((XN3 * X3) * ((XN4 * X4) * ((XN5 * X5) * ((XN6 * X6) * ((XN7 * X7) * ((XN8 * X8) * ((XN9 * X9) * ((XN10 * X10) * ((XN11 * X11) * ((XN12 * X12) * X13)))))))))))),
-	exists xn1 x1 xn2 x2 xn3 x3 xn4 x4 xn5 x5 xn6 x6 xn7 x7 xn8 x8 xn9 x9 xn10 x10 xn11 x11 xn12 x12 x13, p = ((xn1, x1), ((xn2, x2), ((xn3, x3), ((xn4, x4), ((xn5, x5), ((xn6, x6), ((xn7, x7), ((xn8, x8), ((xn9, x9), ((xn10, x10), ((xn11, x11), ((xn12, x12), x13)))))))))))).
-Proof. intros. repeat destruct_prod. repeat eexists. Qed.
-
-Ltac destruct_varname12 :=
-	match goal with
-	| [ H : VARNAME (_) * _ * (VARNAME (_) * _ * (VARNAME (_) * _ * (VARNAME (_) * _ * (VARNAME (_) * _ * (VARNAME (_) * _ * (VARNAME (_) * _ * (VARNAME (_) * _ * (VARNAME (_) * _ * (VARNAME (_) * _ * (VARNAME (_) * _ * ((VARNAME (_) * _) * _))))))))))) |- _ ] =>
-		let Hx := fresh in
-		pose proof (destruct_varname12 H) as Hx;
-		match type of Hx with
-		| exists (_ : VARNAME (vn1)) _ (_ : VARNAME (vn2)) _ (_ : VARNAME (vn3)) _ (_ : VARNAME (vn4)) _ (_ : VARNAME (vn5)) _ (_ : VARNAME (vn6)) _ (_ : VARNAME (vn7)) _ (_ : VARNAME (vn8)) _ (_ : VARNAME (vn9)) _ (_ : VARNAME (vn10)) _ (_ : VARNAME (vn11)) _ (_ : VARNAME (vn12)) _ _ , _ = _ =>
-			destruct Hx as [? [?vn1 [? [?vn2 [? [?vn3 [? [?vn4 [? [?vn5 [? [?vn6 [? [?vn7 [? [?vn8 [? [?vn9 [? [?vn10 [? [?vn11 [? [?vn12 [? Hx] ] ] ] ] ] ] ] ] ] ] ] ] ] ] ] ] ] ] ] ] ] ] ] ]
-		end
-	end.
-
-Theorem destruct_varname14 : forall XN1 X1 XN2 X2 XN3 X3 XN4 X4 XN5 X5 XN6 X6 XN7 X7 XN8 X8 XN9 X9 XN10 X10 XN11 X11 XN12 X12 XN13 X13 XN14 X14 X15 
-				(p : (XN1 * X1) * ((XN2 * X2) * ((XN3 * X3) * ((XN4 * X4) * ((XN5 * X5) * ((XN6 * X6) * ((XN7 * X7) * ((XN8 * X8) * ((XN9 * X9) * ((XN10 * X10) * ((XN11 * X11) * ((XN12 * X12) * ((XN13 * X13) * ((XN14 * X14) * X15)))))))))))))),
-	exists xn1 x1 xn2 x2 xn3 x3 xn4 x4 xn5 x5 xn6 x6 xn7 x7 xn8 x8 xn9 x9 xn10 x10 xn11 x11 xn12 x12 xn13 x13 xn14 x14 x15, p = ((xn1, x1), ((xn2, x2), ((xn3, x3), ((xn4, x4), ((xn5, x5), ((xn6, x6), ((xn7, x7), ((xn8, x8), ((xn9, x9), ((xn10, x10), ((xn11, x11), ((xn12, x12), ((xn13, x13), ((xn14, x14), x15)))))))))))))).
-Proof. intros. repeat destruct_prod. repeat eexists. Qed.
-
-Ltac destruct_varname14 :=
-	match goal with
-	| [ H : VARNAME (_) * _ * (VARNAME (_) * _ * (VARNAME (_) * _ * (VARNAME (_) * _ * (VARNAME (_) * _ * (VARNAME (_) * _ * (VARNAME (_) * _ * (VARNAME (_) * _ * (VARNAME (_) * _ * (VARNAME (_) * _ * (VARNAME (_) * _ * (VARNAME (_) * _ * (VARNAME (_) * _ * ((VARNAME (_) * _) * _))))))))))))) |- _ ] =>
-		let Hx := fresh in
-		pose proof (destruct_varname14 H) as Hx;
-		match type of Hx with
-		| exists (_ : VARNAME (vn1)) _ (_ : VARNAME (vn2)) _ (_ : VARNAME (vn3)) _ (_ : VARNAME (vn4)) _ (_ : VARNAME (vn5)) _ (_ : VARNAME (vn6)) _ (_ : VARNAME (vn7)) _ (_ : VARNAME (vn8)) _ (_ : VARNAME (vn9)) _ (_ : VARNAME (vn10)) _ (_ : VARNAME (vn11)) _ (_ : VARNAME (vn12)) _ (_ : VARNAME (vn13)) _ (_ : VARNAME (vn14)) _ _ , _ = _ =>
-			destruct Hx as [? [?vn1 [? [?vn2 [? [?vn3 [? [?vn4 [? [?vn5 [? [?vn6 [? [?vn7 [? [?vn8 [? [?vn9 [? [?vn10 [? [?vn11 [? [?vn12 [? [?vn13 [? [?vn14 [? Hx] ] ] ] ] ] ] ] ] ] ] ] ] ] ] ] ] ] ] ] ] ] ] ] ] ] ] ] ]
-		end
-	end.
 
 Theorem destruct_varname16 : forall XN1 X1 XN2 X2 XN3 X3 XN4 X4 XN5 X5 XN6 X6 XN7 X7 XN8 X8 XN9 X9 XN10 X10 XN11 X11 XN12 X12 XN13 X13 XN14 X14 XN15 X15 XN16 X16 X17 
 				(p : (XN1 * X1) * ((XN2 * X2) * ((XN3 * X3) * ((XN4 * X4) * ((XN5 * X5) * ((XN6 * X6) * ((XN7 * X7) * ((XN8 * X8) * ((XN9 * X9) * ((XN10 * X10) * ((XN11 * X11) * ((XN12 * X12) * ((XN13 * X13) * ((XN14 * X14) * ((XN15 * X15) * ((XN16 * X16) * X17)))))))))))))))),
@@ -227,4 +165,4 @@ Ltac destruct_varname16 :=
 	end.
 
 Ltac destruct_varnames :=
-	repeat (( destruct_varname16 || destruct_varname14 || destruct_varname12 || destruct_varname10 || destruct_varname8 || destruct_varname6 || destruct_varname4 || destruct_varname2 || destruct_varname1); subst).
+	repeat (( destruct_varname16 ||  destruct_varname8 || destruct_varname4 || destruct_varname2 || destruct_varname1); subst).
