src/HoareL1.v
@@ -1,0 +1,405 @@
+Require Import List BaseTypes Layer1 ProgAuto CommonAutomation.
+Require Import Disk Memx Predx SepAuto Simulation.
+Import ListNotations.
+
+Set Implicit Arguments.
+
+
+(** ** Hoare logic *)
+Definition precond := oracle -> @pred addr addr_dec (set value).
+Definition postcond {T: Type} := oracle ->
+                                 oracle -> T -> @pred addr addr_dec (set value).
+Definition crashcond := oracle ->
+                        oracle ->  @pred addr addr_dec (set value).
+
+
+Definition hoare_triple {T: Type} (pre: precond) (p: prog T) (post: @postcond T) (crash: crashcond):=
+  forall o d ret,
+    pre o d ->
+    exec (o, d) p ret ->
+    ((exists o' d' r,
+         ret = Finished (o', d') r
+         /\ post o o' r d') \/
+     (exists o' d',
+        ret = Crashed (o', d') /\ crash o o' d'))%type.
+
+
+  
+Notation
+  "<< o >> pre p << o' , r >> post crash" :=
+  (forall F, hoare_triple
+          (fun (o:oracle) => F * pre)%pred
+          p
+          (fun (o:oracle) (o':oracle) r => F * post)%pred
+          (fun (o:oracle) o' => F * crash)%pred)
+    (at level 10, o at next level, pre at next level, p at next level, o' at next level,  r at next level, post at next level, crash at next level,
+     format "'[v' '[  ' '<<' o '>>' '//' '[' pre ']' '//' '[' p ']' ']' '//' '[  ' '<<' o' ','  r '>>' '//' '[' post ']' '//' '[' crash ']' ']' ']'").
+
+Notation
+  "{{ e1 }} << o >> pre p << o' , r >> post crash" :=
+   (exists e1, (forall F, hoare_triple
+          (fun (o:oracle) => F * pre)%pred
+          p
+          (fun (o:oracle) (o':oracle) r => F * post)%pred
+          (fun (o:oracle) o' => F * crash)%pred))
+    (at level 10, o at next level, pre at next level, p at next level, o' at next level, r at next level, post at next level, crash at next level,
+     format "'[v' '{{' e1 '}}' '//' '[  ' '<<' o '>>' '//' pre '//' p ']' '//' '[  ' '<<' o' ','  r '>>' '//' post '//' crash ']' ']'").
+
+
+Theorem hoare_triple_strengthen_pre:
+  forall T (p: prog T) (pre pre': precond) post crash,
+  hoare_triple pre p post crash ->
+  (forall o, pre' o =p=>  pre o) ->
+  hoare_triple pre' p post crash.
+Proof.
+  unfold hoare_triple; intros;
+    edestruct H; intros; eauto.
+  eapply H0; eauto.
+Qed.
+
+
+Theorem hoare_triple_weaken_post_weak:
+  forall T (p: prog T) pre (post post': postcond) crash,
+  hoare_triple pre p post crash ->
+  (forall  o d o' r,
+      pre o d ->
+      post o o' r =p=>
+      post' o o' r) ->
+  hoare_triple pre p post' crash.
+Proof.
+  unfold hoare_triple; intros;
+    edestruct H; intros; eauto.
+  cleanup.
+  left; repeat eexists; eauto.
+  eapply H0; eauto.
+Qed.
+
+
+Theorem hoare_triple_weaken_post_strong:
+  forall T (p: prog T) pre (post post': postcond) crash,
+  hoare_triple pre p post crash ->
+  (forall  o o' (r: T),
+      post o o' r =p=>
+      post' o o' r) ->
+  hoare_triple pre p post' crash.
+Proof.
+  intros; eapply hoare_triple_weaken_post_weak; eauto.
+Qed.
+
+Theorem hoare_triple_weaken_crash_weak:
+  forall T (p: prog T) pre post (crash crash': crashcond),
+  hoare_triple pre p post crash ->
+  (forall  o d o',
+      pre o d ->
+      crash o o' =p=>
+      crash' o o') ->
+  hoare_triple pre p post crash'.
+Proof.
+  unfold  hoare_triple; intros;
+    edestruct H; intros; eauto.
+  cleanup.
+  right; repeat eexists; eauto.
+  eapply H0; eauto.
+Qed.
+
+
+Theorem hoare_triple_weaken_crash_strong:
+  forall T (p: prog T) pre post (crash crash': crashcond),
+  hoare_triple pre p post crash ->
+  (forall o o', crash o o' =p=> crash' o o') ->
+  hoare_triple pre p post crash'.
+Proof.
+  intros; eapply hoare_triple_weaken_crash_weak; eauto.
+Qed.
+
+
+Theorem hoare_triple_pimpl_strong :
+    forall T1 T2 (p1: prog T1) (p2: T1 -> prog T2) pre1 pre2 post1 post2 crash1 crash2,
+      hoare_triple pre1 p1 post1 crash1 ->
+      (forall r, hoare_triple pre2 (p2 r) post2 crash2) ->
+    (forall o d o' d' r,
+      pre1 o d ->
+      exec (o, d) p1 (Finished (o', d') r) ->
+      post1 o o' r d' ->
+      pre2 o' d') ->
+    (forall o d o' d',
+      pre1 o d ->
+      exec (o, d) p1 (Crashed (o', d')) ->
+      crash1 o o' d' ->
+      crash2 o o' d') ->
+    (forall o o' d' o'' d'' r r2,
+      post1 o o' r d' ->
+      pre2 o' d' ->
+      exec (o', d') (p2 r) (Finished (o'', d'') r2) ->
+      post2 o o'' r2 d'') ->
+    (forall o o' d' o'' d'' r,
+      post1 o o' r d' ->
+      pre2 o' d' ->
+      exec (o', d') (p2 r) (Crashed (o'', d'')) ->
+      crash2 o o'' d'') ->
+    hoare_triple pre1 (Bind p1 p2) post2 crash2.
+Proof.
+  unfold hoare_triple; intros.
+  invert_exec.
+  {
+    edestruct H; eauto; cleanup.
+    edestruct H0; eauto; cleanup.
+    left; repeat eexists; eauto.
+  }
+  {
+    destruct H6; cleanup;
+    edestruct H; eauto; cleanup.
+    - right; repeat eexists; eauto.
+    - edestruct H0; eauto; cleanup.
+      right; repeat eexists; eauto.
+  }
+  {
+    destruct H6; cleanup;
+    edestruct H; eauto; cleanup;
+    edestruct H0; eauto; cleanup.
+  }
+Qed.
+
+(*
+Theorem hoare_triple_pimpl' :
+    forall T1 T2 (p1: prog T1) (p2: T1 -> prog T2) pre1 post1 post2 crash1 crash2,
+      hoare_triple pre1 p1 post1 crash1 ->
+      (forall r, hoare_triple (fun u o' s' => exists o s d, [[pre1 u o s d]] * post1 u o s o' s' r)%pred (p2 r) post2 crash2) ->
+    (forall u o d s o' d' s' tr,
+      pre1 u o s d ->
+      exec (u, o, d, s) p1 (Crashed (u, o', d', s')) tr ->
+      crash1 u o s o' s' d' ->
+      crash2 u o s o' s' d') ->
+    (forall  u o s o' d' s' o'' s'' d'' r r2 tr,
+      post1 u o s o' s' r d' ->
+      exec (u, o', d', s') (p2 r) (Finished (u, o'', d'', s'') r2) tr ->
+      post2 u o s o'' s'' r2 d'') ->
+    (forall  u o s o' d' s' o'' s'' d'' r tr,
+      post1 u o s o' s' r d' ->
+      exec (u, o', d', s') (p2 r) (Crashed (u, o'', d'', s'')) tr ->
+      crash2 u o s o'' s'' d'') ->
+    hoare_triple pre1 (Bind p1 p2) post2 crash2.
+Proof.
+  unfold hoare_triple; intros.
+  invert_exec.
+  {
+      edestruct H; eauto.
+      destruct H7; cleanup.
+      edestruct H0; eauto.
+      pred_apply; cancel; eauto.
+      destruct H7; eauto; cleanup; eauto.
+      split. left.
+      repeat eexists; eauto.
+      apply trace_ok_app_merge; eauto.
+    }
+    {
+      destruct H5.
+      - edestruct H; eauto; destruct H6; cleanup.
+        split; eauto; right; repeat eexists; eauto.
+      - cleanup.
+        edestruct H; eauto; destruct H7; cleanup.
+        edestruct H0; eauto.
+        pred_apply; cancel; eauto.
+        destruct H7; eauto; cleanup; eauto.
+        split. right.
+        repeat eexists; eauto.
+        apply trace_ok_app_merge; eauto.
+    }
+Qed.
+
+Theorem hoare_triple_pimpl'' :
+    forall T1 T2 (p1: prog T1) (p2: T1 -> prog T2) pre1 post1 post2 crash1 crash2,
+      hoare_triple pre1 p1 post1 crash1 ->
+      (forall u o s d r,
+          pre1 u o s d ->
+          hoare_triple (fun u' o' s' => [[u = u']] * post1 u' o s o' s' r)%pred (p2 r) post2 crash2) ->
+    (forall u o d s o' d' s' tr,
+      pre1 u o s d ->
+      exec (u, o, d, s) p1 (Crashed (u, o', d', s')) tr ->
+      crash1 u o s o' s' d' ->
+      crash2 u o s o' s' d') ->
+    (forall  u o s o' d' s' o'' s'' d'' r r2 tr,
+      post1 u o s o' s' r d' ->
+      exec (u, o', d', s') (p2 r) (Finished (u, o'', d'', s'') r2) tr ->
+      post2 u o s o'' s'' r2 d'') ->
+    (forall  u o s o' d' s' o'' s'' d'' r tr,
+      post1 u o s o' s' r d' ->
+      exec (u, o', d', s') (p2 r) (Crashed (u, o'', d'', s'')) tr ->
+      crash2 u o s o'' s'' d'') ->
+    hoare_triple pre1 (Bind p1 p2) post2 crash2.
+Proof.
+  unfold hoare_triple; intros.
+  invert_exec.
+  {
+      edestruct H; eauto.
+      destruct H7; cleanup.
+      edestruct H0; eauto.
+      pred_apply; cancel; eauto.
+      destruct H7; eauto; cleanup; eauto.
+      split. left.
+      repeat eexists; eauto.
+      apply trace_ok_app_merge; eauto.
+    }
+    {
+      destruct H5.
+      - edestruct H; eauto; destruct H6; cleanup.
+        split; eauto; right; repeat eexists; eauto.
+      - cleanup.
+        edestruct H; eauto; destruct H7; cleanup.
+        edestruct H0; eauto.
+        pred_apply; cancel; eauto.
+        destruct H7; eauto; cleanup; eauto.
+        split. right.
+        repeat eexists; eauto.
+        apply trace_ok_app_merge; eauto.
+    }
+Qed.
+*)
+
+Theorem hoare_triple_pimpl :
+    forall T1 T2 (p1: prog T1) (p2: T1 -> prog T2) pre1 post1 post2 crash1 crash2,
+      hoare_triple pre1 p1 post1 crash1 ->
+      (forall o d r,
+          pre1 o d ->
+          hoare_triple (fun o' => post1 o o' r)%pred (p2 r) post2 crash2) ->
+    (forall o d o',
+      pre1 o d ->
+      crash1 o o' =p=> crash2 o o') ->
+    (forall o d o' d' o'' r r2,
+      pre1 o d ->
+      post1 o o' r d' ->
+      post2 o' o'' r2 =p=> post2 o o'' r2) ->
+    (forall o d o' d' o'' r,
+      pre1 o d ->
+      post1 o o' r d' ->
+      crash2 o' o'' =p=> crash2 o o'') ->
+    hoare_triple pre1 (Bind p1 p2) post2 crash2.
+Proof.
+  unfold hoare_triple; intros.
+  invert_exec.
+  {
+    edestruct H; eauto; cleanup;
+    edestruct H0; eauto; cleanup.
+    left; repeat eexists; eauto.
+    eapply H2; eauto.
+  }
+  {
+    destruct H5; cleanup;
+    edestruct H; eauto; cleanup.
+    - right; repeat eexists; eauto.
+      eapply H1; eauto.
+    - edestruct H0; eauto; cleanup.
+      right; repeat eexists; eauto.
+      eapply H3; eauto.
+  }
+  {
+    destruct H5; cleanup;
+    edestruct H; eauto; cleanup;
+    edestruct H0; eauto; cleanup.
+  }
+Qed.
+
+
+
+Theorem hoare_triple_equivalence :
+  forall T (p p': prog T) pre post crash,
+    hoare_triple pre p post crash ->
+    prog_equiv p p' ->
+    hoare_triple pre p' post crash.
+Proof.
+  unfold hoare_triple; intros.
+  edestruct H; eauto; cleanup.
+  match goal with
+  | [ H: _ ~= _ |- _ ] =>
+    edestruct H; eauto
+  end.
+Qed.
+
+
+Ltac monad_simpl_one :=
+  match goal with
+  | [ |- hoare_triple _ (Bind (Bind _ _) _) _ _ ] =>
+    eapply hoare_triple_equivalence;
+    [ | apply bind_assoc ]
+  end.
+
+Ltac monad_simpl := repeat monad_simpl_one.
+
+
+Lemma deterministic_prog:
+  forall T (p: prog T) st ret1 ret2,
+    exec st p ret1 ->
+    exec st p ret2 ->
+    ret1 = ret2.
+Proof.
+  unfold state; induction p; simpl; intros;
+  invert_exec; cleanup;
+    invert_exec; cleanup;
+      destruct_pairs; cleanup; eauto.
+  
+  specialize IHp with (1:= H0)(2:=H1); cleanup.
+  specialize H with (1:= H2)(2:=H3); cleanup.
+  eauto.
+  
+  destruct H0; cleanup.
+  specialize IHp with (1:= H0)(2:=H1); cleanup.
+  specialize IHp with (1:= H0)(2:=H1); cleanup.
+  specialize H with (1:= H2)(2:=H3); cleanup.
+
+  destruct H0; cleanup.
+  specialize IHp with (1:= H0)(2:=H1); cleanup.
+  specialize IHp with (1:= H0)(2:=H1); cleanup.
+  specialize H with (1:= H2)(2:=H3); cleanup.
+  
+  destruct H1; cleanup.
+  specialize IHp with (1:= H0)(2:=H1); cleanup.
+  specialize IHp with (1:= H0)(2:=H1); cleanup.
+  specialize H with (1:= H2)(2:=H3); cleanup.
+
+  destruct H0; cleanup; destruct H1; cleanup.
+  specialize IHp with (1:= H0)(2:=H1); cleanup; eauto.
+  
+  specialize IHp with (1:= H0)(2:=H1); cleanup.
+
+  specialize IHp with (1:= H0)(2:=H1); cleanup.
+
+  specialize IHp with (1:= H0)(2:=H1); cleanup.
+  specialize H with (1:= H2)(2:=H3); cleanup.
+  eauto.
+
+  destruct H0; cleanup; destruct H1; cleanup.
+  specialize IHp with (1:= H0)(2:=H1); cleanup; eauto.
+  
+  specialize IHp with (1:= H0)(2:=H1); cleanup.
+
+  specialize IHp with (1:= H0)(2:=H1); cleanup.
+
+  specialize IHp with (1:= H0)(2:=H1); cleanup.
+  specialize H with (1:= H2)(2:=H3); cleanup.
+
+  destruct H1; cleanup.
+  specialize IHp with (1:= H0)(2:=H1); cleanup.
+  specialize IHp with (1:= H0)(2:=H1); cleanup.
+  specialize H with (1:= H2)(2:=H3); cleanup.
+  
+  destruct H0; cleanup; destruct H1; cleanup.
+  specialize IHp with (1:= H0)(2:=H1); cleanup; eauto.
+  
+  specialize IHp with (1:= H0)(2:=H1); cleanup.
+
+  specialize IHp with (1:= H0)(2:=H1); cleanup.
+
+  specialize IHp with (1:= H0)(2:=H1); cleanup.
+  specialize H with (1:= H2)(2:=H3); cleanup.
+
+  destruct H0; cleanup; destruct H1; cleanup.
+  specialize IHp with (1:= H0)(2:=H1); cleanup; eauto.
+  
+  specialize IHp with (1:= H0)(2:=H1); cleanup.
+
+  specialize IHp with (1:= H0)(2:=H1); cleanup.
+
+  specialize IHp with (1:= H0)(2:=H1); cleanup.
+  specialize H with (1:= H2)(2:=H3); cleanup.
+  eauto.
+Qed.
