src/Layer1.v
@@ -1,0 +1,86 @@
+Require Import List BaseTypes Memx CommonAutomation Disk Simulation.
+Import ListNotations.
+
+Set Implicit Arguments.
+
+Section Layer1.
+
+  Definition state := (oracle * (disk value))%type.
+  Definition get_oracle (st: state) := fst st.
+  Definition get_disk (st: state) := snd st.
+  
+  Inductive prog : Type -> Type :=
+  | Read : addr -> prog value
+  | Write : addr -> value -> prog unit
+  | Ret : forall T, T -> prog T
+  | Bind : forall T T', prog T -> (T -> prog T') -> prog T'.
+   
+  Inductive exec :
+    forall T, state -> prog T -> @Result state T -> Prop :=
+  | ExecRead : 
+      forall st o' a v,
+        let o := fst st in
+        let d := snd st in
+        o = Cont::o' ->
+        read d a = Some v ->
+        exec st (Read a) (Finished (o', d) v)
+             
+  | ExecWrite :
+      forall st o' a v,
+        let o := fst st in
+        let d := snd st in
+        o = Cont::o' ->
+        read d a <> None ->
+        exec st (Write a v) (Finished (o', (write d a v)) tt)
+             
+  | ExecRet :
+      forall st o' T (v: T),
+        let o := fst st in
+        let d := snd st in
+        o = Cont::o' ->
+        exec st (Ret v) (Finished (o', d) v)
+
+  | ExecBind :
+      forall T T' (p1: prog T) (p2: T -> prog T')
+        st st1 r ret,
+        exec st p1 (Finished st1 r) ->
+        exec st1 (p2 r) ret ->
+        exec st (Bind p1 p2) ret
+
+  | ExecReadCrash :
+      forall st o' a,
+        let o := fst st in
+        let d := snd st in
+        o = Crash::o' ->
+        exec st (Read a) (Crashed (o', d))
+             
+  | ExecWriteCrash :
+      forall st o' a v,
+        let o := fst st in
+        let d := snd st in
+        o = Crash::o' ->
+        exec st (Write a v) (Crashed (o', d))
+             
+  | ExecRetCrash :
+      forall st o' T (v: T),
+        let o := fst st in
+        let d := snd st in
+        o = Crash::o' ->
+        exec st (Ret v) (Crashed (o', d))
+             
+  | ExecBindCrash :
+      forall T T' (p1: prog T) (p2: T -> prog T')
+        st st1,
+        exec st p1 (Crashed st1) ->
+        exec st (Bind p1 p2) (Crashed st1)
+
+  | ExecBindFail :
+      forall T T' (p1: prog T) (p2: T -> prog T')
+        st st1,
+        exec st p1 (Failed st1) ->
+        exec st (Bind p1 p2) (Failed st1).
+  (* TODO: add Failed cases *)
+  
+End Layer1.
+
+Notation "x <- p1 ; p2" := (Bind p1 (fun x => p2))(right associativity, at level 60).
