src/OpSpec.v
@@ -1,17 +1,14 @@
 Require Import List BaseTypes Memx Predx.
-Require Import CommonAutomation SepAuto Prog ProgAuto Hoare.
+Require Import CommonAutomation SepAuto Layer1 ProgAuto HoareL1.
 Open Scope pred_scope.
 
 Theorem read_okay:
   forall a v,
-    << u, o, s >>
+    << o >>
      (a |-> v)
      (Read a)
-    << o', s', r >>
-     ([[o = Handle r :: o']] *
-      [[s r = None]] *
-      [[s' = upd s r (fst v)]] *
-      a |-> v)
+    << o', r >>
+     (a |-> v * [[r = fst v]])
      (a |-> v).
 Proof.
   intros.
@@ -19,28 +16,25 @@ Proof.
   destruct_lift H; subst.
   invert_exec; cleanup.
   {
-    split; [|simpl]; auto; left.
-    do 4 eexists; split; eauto.
+    left.
+    do 3 eexists; split; eauto.
     unfold Disk.read in *;
     eapply ptsto_valid' in H as Hx;
     cleanup; eauto.  
-    unfold Disk.upd_store.
     simpl in *; pred_apply; cancel; eauto.
   }
   {
-    split; [|simpl]; auto; right; eauto.
+    simpl in *; cleanup; right; eauto.
   }
 Qed.
 
 Theorem write_okay:
-  forall a h v v',
-    << u, o, s >>
-     ([[s h = Some v' ]] * a |-> v)
-     (Write a h)
-    << o', s', r >>
-     ([[s' = s]] *
-      [[o' = o]] *
-      a |-> (v', (fst v::snd v)))
+  forall a v v',
+    << o >>
+     (a |-> v)
+     (Write a v')
+    << o', r >>
+     (a |-> (v', (fst v::snd v)))
      (a |-> v).
 Proof.
   intros.
@@ -48,144 +42,40 @@ Proof.
   destruct_lift H; subst.
   invert_exec; cleanup; simpl in *.
   {
-    split; [|simpl]; auto; left.
-    do 4 eexists; split; eauto.
+    left.
+    do 3 eexists; split; eauto.
     unfold Disk.read in *;
     eapply ptsto_valid' in H as Hx;
     cleanup; eauto.  
     unfold Disk.write; cleanup.
     unfold Disk.upd_disk.
-    apply sep_star_assoc.
     eapply ptsto_upd'.
     pred_apply; cancel; eauto.
   }
   {
-    split; [|simpl]; auto; right; eauto.
-  }
-Qed.
-
-Theorem write_okay_any:
-  forall P a h v,
-    << u, o, s >>
-     ([[s h = None ]] * a |-> v)
-     (Write a h)
-    << o', s', r >>
-     (P)
-     (a |-> v).
-Proof.
-  intros.
-  unfold hoare_triple; intros.
-  destruct_lift H; subst.
-  invert_exec; cleanup; simpl in *.
-  cleanup.
-  split; [|simpl]; auto; right; eauto.
-Qed.
-
-Theorem auth_okay:
-  forall p,
-    << u, o, s >>
-     [[True]]
-     (Auth p)
-    << o', s', r >>
-     ([[s' = s]] *
-      [[o' = o]] *
-      [[(r = true /\ can_access u p) \/
-       (r = false /\ ~can_access u p)]])
-     [[True]].
-Proof.
-  intros.
-  unfold hoare_triple; intros.
-  invert_exec; cleanup; simpl in *.
-  {
-    split; [|simpl]; auto; left.
-    do 4 eexists; split; eauto.
-    pred_apply; cancel; eauto.
-  }
-  {
-    split; [|simpl]; auto; left.
-    do 4 eexists; split; eauto.
-    pred_apply; cancel; eauto.
-  }
-  {
-    split; [|simpl]; auto; right; eauto.
-  }
-Qed.
-
-Theorem seal_okay:
-  forall p v,
-    << u, o, s >>
-     [[True]]
-     (Seal p v)
-    << o', s', r >>
-     ([[o = Handle r :: o']] *
-      [[s r = None]] *
-      [[s' = upd s r (p,v)]])
-     [[True]].
-Proof.
-  intros.
-  unfold hoare_triple; intros.
-  invert_exec; cleanup; simpl in *.
-  {
-    split; [|simpl]; auto; left.
-    do 4 eexists; split; eauto.
-    pred_apply; cancel; eauto.
-  }
-  {
-    split; [|simpl]; auto; right; eauto.
-  }
-Qed.
-
-
-Theorem unseal_okay:
-  forall h v,
-    << u, o, s >>
-     ([[s h = Some v]] *
-      [[can_access u (fst v)]])           
-     (Unseal h)
-    << o', s', r >>
-     ([[o' = o]] *
-      [[s' = s]] *
-      [[r = snd v]])
-     [[True]].
-Proof.
-  intros.
-  unfold hoare_triple; intros.
-  destruct_lift H.
-  invert_exec; cleanup; simpl in *; cleanup.
-  {
-    split; [|simpl]; eauto; left.
-    do 4 eexists; split; eauto.
-    pred_apply; cancel; eauto.
-  }
-  {
-    split; [|simpl]; auto; right; eauto.
-    do 3 eexists;
-      split; eauto.
-    pred_apply; cancel.
+    simpl in *; cleanup; right; eauto. 
   }
 Qed.
 
 Theorem ret_okay:
   forall T (v: T),
-    << u, o, s >>
-     [[True]]
+    << o >>
+     emp
      (Ret v)
-    << o', s', r >>
-     ([[o' = o]] *
-      [[s' = s]] *
-      [[r = v]])
-     [[True]].
+    << o', r >>
+     (emp * [[r = v]])
+     emp.
 Proof.
   intros.
   unfold hoare_triple; intros.
   invert_exec; cleanup; simpl in *.
   {
-    split; [|simpl]; auto; left.
-    do 4 eexists; split; eauto.
+    left.
+    do 3 eexists; split; eauto.
     pred_apply; cancel; eauto.
   }
   {
-    split; [|simpl]; auto; right; eauto.
+    simpl in *; cleanup; right; eauto.
   }
 Qed.
 
