src/SepAuto.v
@@ -669,7 +669,7 @@ Ltac destruct_pair_eq :=
     end.
 
 Ltac norml := 
-             norm'l; repeat deex; repeat destruct_type valueset;
+             norm'l; repeat deex; repeat destruct_type set;
              repeat destruct_pair_eq;
              (* To check whether [split_or_l] succeeded, we require that it
               * produce at least 2 subgoals.  Also, because [split_or_l] reverses
